finish gcd proofs

lib/gcd.dfy
@@ -6,7 +6,28 @@ module Math {
     }
 
     ghost function Factors(x: pos): set<pos> {
-        set p: pos | p <= x  && IsFactor(p, x)  // error: set constructed must be finite
+        set p: pos | p <= x  && IsFactor(p, x)
+    }
+
+    ghost predicate IsFactorNat(p: nat, x: nat) {
+        exists q: nat ::  p * q == x
+    }
+
+    ghost function FactorsNat(x: nat): set<nat> {
+        set p: nat | p <= x  && IsFactorNat(p, x)
+    }
+
+    lemma FactorsNatNotZero(x: nat)
+        requires x!=0
+        ensures forall y :: y in FactorsNat(x) ==> y > 0
+    {}
+
+
+    lemma FactorsNatEquiv(x: nat)
+        requires x!=0
+        ensures FactorsNat(x) == Factors(x)
+    {
+        
     }
 
     lemma FactorIsFactorOfLinearCombination(a: pos, b: pos, c: pos)
@@ -324,6 +345,9 @@ module Math {
         }
     }
 
+    lemma FactorsMult(x: pos, y: pos)
+        ensures Factors(x*y) == set d_x, d_y | d_x in Factors(x) && d_y in Factors(y) :: d_x * d_y
+
     lemma Divides(p: pos, y: pos, x: pos)
         requires x in Factors(p*y)
         // requires IsFactor(x ,p*y)
@@ -360,6 +384,7 @@ module Math {
         requires Gcd(x,y) * s == x
         requires Gcd(x,y) * t == y
         ensures Gcd(s,t) == 1
+        ensures Factors(s) * Factors(t) == {1}
     {
         assert s * Gcd(x,y) == x;
         assert IsFactor(s, x);
@@ -384,50 +409,41 @@ module Math {
             assert IsFactor(Gcd(x,y)*Gcd(s,t), y);
             assert false;
         }
+        FactorsContains1(s);
+        FactorsContains1(t);
+        if Factors(s) * Factors(t) != {1} {
+            assert Factors(s) * Factors(t) != {};
+            var x :| x in Factors(s) * Factors(t) && x != 1;
+            assert false;
+        }
     }
 
-    lemma {:verify } {:vcs_split_on_every_assert} GcdFactors(x: pos, y: pos)
+    lemma GcdFactors(x: pos, y: pos)
         ensures Factors(x) * Factors(y) == Factors(Gcd(x,y))
     {
         AboutGcd(x,y);
         FactorsContainsSelf(Gcd(x,y));
-        assert Gcd(x,y) <= x;
-        assert Gcd(x,y) <= y;
+        // assert Gcd(x,y) <= x;
+        // assert Gcd(x,y) <= y;
         var s :| Gcd(x,y) * s == x;
-        assert s * Gcd(x,y) == x;
+        // assert s * Gcd(x,y) == x;
         var t :| Gcd(x,y) * t == y;
-        assert t * Gcd(x,y) == y;
-        GcdRest(x,y, s, t);
+        // assert t * Gcd(x,y) == y;
+        // GcdRest(x,y, s, t);
         assert forall p: pos :: p in Factors(x)*Factors(y) ==> p in Factors(Gcd(x,y)) by {
             forall p: pos | p in Factors(x)*Factors(y)
                 ensures p in Factors(Gcd(x,y))
             {
-                var q: pos :| p * q == x;
-                var r: pos :| p * r == y;
-                assert r *p ==y;
-                assert q * p == x;
-                assert IsFactor(q, x);
-                assert IsFactor(s, x);
-                assert IsFactor(t, y);
-                assert IsFactor(r, y);
-                assert p <= Gcd(x,y);
+                // assert IsFactor(s, x);
+                // assert IsFactor(t, y);
+                // assert p <= Gcd(x,y);
                 assert IsFactor(p, Gcd(x,y)) by {
-                    if p == Gcd(x,y) {
-                    }else{
-                        if !IsFactor(p, Gcd(x,y)) {
-                            calc {
-                                p * q;
-                                Gcd(x,y)*s;
-                            }
-                            assert p*q/s == Gcd(x,y);
-                            calc {
-                                p*r;
-                                Gcd(x,y)*t;
-                            }
-                            assert p*r/t == Gcd(x,y);
-                         assert false;   
-                        }
-                    }
+                    AboutEuclid2(x, y);
+                    FactorsNatEquiv(x);
+                    FactorsNatEquiv(y);
+                    FactorsNatEquiv(Gcd(x,y));
+                    EuclidGcdEquivalence(x, y);
+                    EuclidGreatest(x, y);
                 }
             }
         }
@@ -536,6 +552,203 @@ module Math {
             // We just showed that q is a common factor of x and y.
             assert q in Factors(x) * Factors(y);
             // By the definition of Gcd(x, y), we then have that q <= p.
+        }
+    }
+
+    function Euclid(x: nat, y: nat): nat 
+        decreases y, x
+    {
+        if y == 0 then 
+            x
+        else
+            Euclid(y, x % y)
+    }
+
+    lemma AboutEuclid(x: nat, y: nat)
+        requires y == 0
+        requires x > 0
+        ensures Euclid(x,y) > 0
+    {}
+
+    lemma AboutEuclid2(x: pos, y: pos)
+        ensures Euclid(x,y) > 0
+    {
+        if x < y {
+            EuclidMod2(x,y);
+
+        }else{
+
+        }
+    }
+
+    lemma EuclidGcdEquivalence(x: pos, y: pos)
+        ensures Euclid(x,y) == Gcd(x,y)
+    {
+        AboutEuclid2(x, y);
+        FactorsNatEquiv(x);
+        FactorsNatEquiv(y);
+        FactorsNatEquiv(Gcd(x,y));
+        AboutGcd(x, y);
+        EuclidGreatest(x, y);
+        EuclidDivisor(x, y);
+        var gcde := Euclid(x, y);
+        var ggcd := Gcd(x, y);
+        assert gcde <= Gcd(x, y);
+        assert gcde >= Gcd(x, y);
+
+    }
+
+    lemma EuclidDivisor(x: pos, y: pos)
+        requires Euclid(x,y) > 0
+        ensures IsFactor(Euclid(x,y), x)
+        ensures IsFactor(Euclid(x,y), y)
+        decreases y,x
+    {
+        if x % y == 0 {
+            calc {
+                Euclid(x,y);
+                Euclid(y, 0);
+                y;
+            }
+            assert y * 1 == y;
+            assert IsFactor(y, y);
+            var k: nat := x / y;
+            assert y * k == x;
+            assert IsFactor(y, x);
+
+        }else{
+            calc {
+                Euclid(x, y);
+                Euclid(y, x%y);
+            }
+            EuclidDivisor(y, x%y);
+            var q :| Euclid(y, x%y) * q == (x%y);
+            var s :| Euclid(y, x%y) * s == y;
+            assert y*(x / y) + x%y == x;
+            calc {
+                x;
+                y*(x / y) + x%y;
+                y*(x / y) + Euclid(y, x%y) * q;
+                (Euclid(y, x%y) * s)*(x / (Euclid(y, x%y) * s)) + Euclid(y, x%y) * q;
+                Euclid(y, x%y) * (s*(x / y) + 1 * q);
+            }
+
+            assert IsFactor(Euclid(x,y), x);
+            assert IsFactor(Euclid(x,y), y);
+        }
+    }
+
+    lemma EuclidSymmetric(x: nat, y: nat)
+        ensures Euclid(x, y) == Euclid(y, x)
+    {
+        if y == 0 {
+
+        }
+    }
+
+    lemma EulerIdempotent(x: nat)
+        ensures Euclid(x,x) == x
+    {}
+
+    lemma EuclidMod2(x: nat, y: nat)
+        requires 0 < x < y
+        ensures Euclid(x, y) == Euclid(x, y % x)
+    { 
+        EuclidSymmetric(x, y);
+    }
+
+    // lemma EulerSubtract(x: nat, y: nat)
+    //     requires x < y
+    //     ensures Euclid(x, y) == Euclid(x, y-x)
+    // {
+    //     var p := Euclid(x, y);
+    // }
+
+    
+    lemma ModLemma(x: nat, y: pos, z: nat)
+        requires IsFactorNat(z, x)
+        requires IsFactorNat(z, y)
+        ensures IsFactorNat(z, x % y)
+    {
+        if x % y == 0 {
+            assert z * 0 == x % y;
+            assert IsFactorNat(z, x % y);
+        }else if x < y {
+
+        }else{
+            assert x > y by {
+                if x == 0 {
+
+                }
+            }
+            var p :| z * p == x;
+            var q :| z * q == y;
+            assert p >= q;
+            // assert p - q * (x/y) > 0;
+            calc {
+                x % y;
+                x - y*(x/y);
+                (z*p) - (z*q)*(x/y);
+                z *(p - q * (x/y));
+            }
+            assert IsFactorNat(z, x);
+        }
+    }
+
+    lemma EuclidMod(x: pos, y: pos)
+        ensures IsFactorNat(Euclid(x, y), x % y)
+    {
+        AboutEuclid2(x, y);
+        EuclidDivisor(x, y);
+        if x % y == 0 {
+            var g: nat := x/y;
+            assert Euclid(x,y) * 0 == x%y;
+
+            assert IsFactorNat(Euclid(x,y), x);
+        } else if x < y {
+            assert x % y == x;
+            assert IsFactorNat(Euclid(x,y), x);
+        }else{
+            assert x > y by {
+                if x == y {
+                }
+            }
+            var p :| Euclid(x,y) * p == x;
+            var q :| Euclid(x,y) * q == y;
+            assert p >= q;
+            assert p - q * (x/y) > 0;
+            calc {
+                x % y;
+                x - y*(x/y);
+                (Euclid(x,y)*p) - (Euclid(x,y)*q)*(x/y);
+                Euclid(x,y) *(p - q * (x/y));
+            }
+            assert IsFactorNat(Euclid(x,y), x);
+        }
+    }
+
+    lemma EuclidGreatest(x: nat, y: nat)
+        ensures forall z :: z in FactorsNat(x)*FactorsNat(y) ==> IsFactorNat(z, Euclid(x,y))
+        decreases y, x
+    {
+        forall z |  z in FactorsNat(x)*FactorsNat(y)
+            ensures IsFactorNat(z, Euclid(x,y))
+        {
+            if y == 0 {
+                assert IsFactorNat(z, Euclid(x,y));
+            }else{
+                if x == 0 {
+                    assert IsFactorNat(z, Euclid(x,y));
+                }else{
+                    assert x > 0;
+                    assert y > 0;
+                    ModLemma(x, y, z);
+                    assert IsFactorNat(z, x % y);
+                    EuclidGreatest(y, x % y);
+
+                }
+
+            }
         }
     }
 
